refactor: cleaning up

src/NFO/Aux.v
@@ -1,28 +1,29 @@
+(* This module contains some auxiliary functions *)
 
+(* Inverts a  *)
+Definition invF {X Y} (f: X -> Y) (y: Y) := exists x, f x = y.
 
-Definition invF {X Y} (f: X -> Y) (x: Y) := exists y, f y = x.
+Definition inv2 {X Y W} (f: X -> W) (g : Y -> W) w :=
+  invF f w \/ invF g w.
 
-Definition inv2 {X Y W} (f: X -> W) (g : Y -> W) x :=
-  invF f x \/ invF g x.
-
-Definition inv3 {X Y Z W} (f: X -> W) (g : Y -> W) (h : Z -> W) x :=
-  invF f x \/ invF g x \/ invF h x.
+Definition inv3 {X Y Z W} (f: X -> W) (g : Y -> W) (h : Z -> W) w :=
+  invF f w \/ invF g w \/ invF h w.
 
 Lemma inv2_1 {X Y W} (f: X -> W) (g : Y -> W) x:
   inv2 f g (f x).
 Proof. unfold inv2. unfold invF. left. exists x. auto. Qed.
-Lemma inv2_2 {X Y W} (f: X -> W) (g : Y -> W) x:
-  inv2 f g (g x).
-Proof. unfold inv2. unfold invF. right. exists x. auto. Qed.
+Lemma inv2_2 {X Y W} (f: X -> W) (g : Y -> W) y:
+  inv2 f g (g y).
+Proof. unfold inv2. unfold invF. right. exists y. auto. Qed.
 Hint Resolve inv2_1. Hint Resolve inv2_2.
 
 Lemma inv3_1 {X Y Z W} (f: X -> W) (g : Y -> W) (h : Z -> W) x:
   inv3 f g h (f x).
 Proof. unfold inv3. unfold invF. left. exists x. auto. Qed.
-Lemma inv3_2 {X Y Z W} (f: X -> W) (g : Y -> W) (h : Z -> W) x:
-  inv3 f g h (g x).
-Proof. unfold inv3. unfold invF. right. left. exists x. auto. Qed.
-Lemma inv3_3 {X Y Z W} (f: X -> W) (g : Y -> W) (h : Z -> W) x:
-  inv3 f g h (h x).
-Proof. unfold inv3. unfold invF. right. right. exists x. auto. Qed.
+Lemma inv3_2 {X Y Z W} (f: X -> W) (g : Y -> W) (h : Z -> W) y:
+  inv3 f g h (g y).
+Proof. unfold inv3. unfold invF. right. left. exists y. auto. Qed.
+Lemma inv3_3 {X Y Z W} (f: X -> W) (g : Y -> W) (h : Z -> W) z:
+  inv3 f g h (h z).
+Proof. unfold inv3. unfold invF. right. right. exists z. auto. Qed.
 Hint Resolve inv3_1. Hint Resolve inv3_2. Hint Resolve inv3_3.
