src/NFO/FunExt.v
@@ -1,8 +1,12 @@
+(* ext f g holds iff f and g are extensionally equal *)
 Definition ext {X Y} f g :=
   forall x: X, f x = (g x : Y).
 
-Definition extP {X} f g :=
-  forall x: X, f x <-> g x.
+(* A weaker version of function extensionality on predicates,
+   using equivalence instead of equality *)
+Definition extP {X} P Q :=
+  forall x: X, P x <-> Q x.
 
-Definition extP2 {X Y} f g :=
-  forall x: X, forall y: Y, f x y <-> g x y.
+(* Extensional binary predicates *)
+Definition extP2 {X Y} P Q :=
+  forall x: X, forall y: Y, P x y <-> Q x y.
